code/sha2-mb/Hacl.Spec.SHA2.Equiv.fst
@@ -8,8 +8,8 @@ open Lib.IntVector
 open Lib.IntVector.Serialize
 open Lib.LoopCombinators
 
-open Hacl.Spec.SHA2.Vec
 open Spec.Hash.Definitions
+open Hacl.Spec.SHA2.Vec
 module Spec = Hacl.Spec.SHA2
 module LSeq = Lib.Sequence
 module BSeq = Lib.ByteSequence
@@ -76,7 +76,7 @@ let seq_of_list_is_create8 #a x0 x1 x2 x3 x4 x5 x6 x7 =
   eq_intro rp lp
 
 
-val shuffle_core_pre_create8: a:sha2_alg -> k_t:word a -> ws_t:word a -> hash:words_state a -> words_state a
+val shuffle_core_pre_create8: a:sha2_alg -> k_t:word a -> ws_t:word a -> hash:words_state' a -> words_state' a
 let shuffle_core_pre_create8 a k_t ws_t hash =
   let a0 = Seq.index hash 0 in
   let b0 = Seq.index hash 1 in
@@ -92,7 +92,7 @@ let shuffle_core_pre_create8 a k_t ws_t hash =
   create8 (t1 +. t2) a0 b0 c0 (d0 +. t1) e0 f0 g0
 
 
-val shuffle_core_pre_create8_lemma: a:sha2_alg -> k_t:word a -> ws_t:word a -> hash:words_state a ->
+val shuffle_core_pre_create8_lemma: a:sha2_alg -> k_t:word a -> ws_t:word a -> hash:words_state' a ->
   Lemma (Spec.shuffle_core_pre a k_t ws_t hash == shuffle_core_pre_create8 a k_t ws_t hash)
 let shuffle_core_pre_create8_lemma a k_t ws_t hash =
   let a0 = Seq.index hash 0 in
@@ -292,13 +292,12 @@ val shuffle_lemma_l:
 let shuffle_lemma_l #a #m ws st l =
   shuffle_loop_lemma #a #m ws st l (Spec.num_rounds16 a)
 
-
 val init_lemma_l: a:sha2_alg -> m:m_spec -> l:nat{l < lanes a m} ->
-  Lemma ((state_spec_v (init a m)).[l] == Spec.init a)
+  Lemma ((state_spec_v (init a m)).[l] == Pervasives.fst (Spec.init a))
 
 let init_lemma_l a m l =
   eq_intro #(word a) #(state_word_length a)
-    (state_spec_v (init a m)).[l] (Spec.init a)
+    (state_spec_v (init a m)).[l] (Pervasives.fst (Spec.init a))
 
 
 val load_blocks_lemma_ij:
@@ -385,12 +384,13 @@ let load_blocks_lemma_ij_subst #a #m b j i =
     }
 
 
+#push-options "--z3rlimit 150"
 val load_ws_lemma_l:
     #a:sha2_alg
   -> #m:m_spec{is_supported a m}
   -> b:multiblock_spec a m
   -> j:nat{j < lanes a m} ->
-  Lemma ((ws_spec_v (load_ws b)).[j] == BSeq.uints_from_bytes_be #(word_t a) #SEC b.(|j|))
+  Lemma ((ws_spec_v (load_ws b)).[j] == BSeq.uints_from_bytes_be #(word_t a) #SEC #block_word_length b.(|j|))
 
 let load_ws_lemma_l #a #m b j =
   let lp = Seq.index (ws_spec_v (load_ws b)) j in
@@ -407,6 +407,7 @@ let load_ws_lemma_l #a #m b j =
 
   Classical.forall_intro aux;
   eq_intro lp rp
+#pop-options
 
 
 val state_spec_v_map2_add:
@@ -431,7 +432,7 @@ val update_lemma_l:
   -> st:state_spec a m
   -> l:nat{l < lanes a m} ->
   Lemma ((state_spec_v (update b st)).[l] ==
-    Spec.update a b.(|l|) (state_spec_v st).[l])
+    Pervasives.fst (Spec.update a b.(|l|) ((state_spec_v st).[l], ())))
 
 let update_lemma_l #a #m b st l =
   reveal_opaque (`%update) (update #a #m);
@@ -473,7 +474,7 @@ val update_last_lemma_l:
   -> st:state_spec a m
   -> l:nat{l < lanes a m} ->
   Lemma ((state_spec_v (update_last totlen len b st)).[l] ==
-    Spec.update_last a totlen len b.(|l|) (state_spec_v st).[l])
+    Pervasives.fst (Spec.update_last a totlen len b.(|l|) ((state_spec_v st).[l], ())))
 
 let update_last_lemma_l #a #m totlen len b st0 l =
   let blocks = padded_blocks a len in
@@ -545,23 +546,22 @@ val store_state_lemma_l:
   -> l:nat{l < lanes a m} ->
   Lemma
    (sub (store_state st) (l * (8 * word_length a)) (8 * word_length a) ==
-    Spec.store_state a (state_spec_v st).[l])
+    Spec.store_state a ((state_spec_v st).[l], ()))
 
 let store_state_lemma_l #a #m st l =
-  let st_l : words_state a = (state_spec_v st).[l] in
+  let st_l : words_state a = (state_spec_v st).[l], () in
   let rp = Spec.store_state a st_l in
   let lp = store_state st in
 
   let aux (i:nat{i < 8 * word_length a}) : Lemma (lp.[l * (8 * word_length a) + i] == rp.[i]) =
     //assert (rp == BSeq.uints_to_bytes_be #(word_t a) #SEC #8 st_l);
-    BSeq.index_uints_to_bytes_be #(word_t a) #SEC #8 st_l i;
-    assert (rp.[i] == (BSeq.uint_to_bytes_be (Seq.index st_l (i / word_length a))).[i % word_length a]);
+    BSeq.index_uints_to_bytes_be #(word_t a) #SEC #8 (Pervasives.fst st_l) i;
     store_state_lemma_ij #a #m st l i in
 
   Classical.forall_intro aux;
   eq_intro
     (sub (store_state st) (l * (8 * word_length a)) (8 * word_length a))
-    (Spec.store_state a (state_spec_v st).[l])
+    (Spec.store_state a ((state_spec_v st).[l], ()))
 
 
 // val emit_lemma_l:
@@ -579,7 +579,7 @@ val finish_lemma_l:
   -> #m:m_spec{is_supported a m}
   -> st:state_spec a m
   -> l:nat{l < lanes a m} ->
-  Lemma ((finish st).(|l|) == Spec.finish a (state_spec_v st).[l])
+  Lemma ((finish st).(|l|) == Spec.finish a ((state_spec_v st).[l], ()))
 
 let finish_lemma_l #a #m st l =
   store_state_lemma_l #a #m st l
@@ -595,7 +595,7 @@ val update_block_lemma_l:
   -> l:nat{l < lanes a m} ->
   Lemma
    ((state_spec_v (update_block len b i st)).[l] ==
-    Spec.update_block a len b.(|l|) i (state_spec_v st).[l])
+    Pervasives.fst (Spec.update_block a len b.(|l|) i ((state_spec_v st).[l], ())))
 
 let update_block_lemma_l #a #m len b i st l =
   let mb = get_multiblock_spec len b i in
@@ -612,23 +612,23 @@ val update_nblocks_loop_lemma:
   -> n:nat{n <= len / block_length a } ->
   Lemma
    ((state_spec_v (repeati n (update_block #a #m len b) st)).[l] ==
-    repeati n (Spec.update_block a len b.(|l|)) (state_spec_v st).[l])
+    Pervasives.fst (repeati n (Spec.update_block a len b.(|l|)) ((state_spec_v st).[l], ())))
 
 let rec update_nblocks_loop_lemma #a #m len b st l n =
   let lp = repeati n (update_block #a #m len b) st in
   let f_sc = Spec.update_block a len b.(|l|) in
-  let rp = repeati n f_sc (state_spec_v st).[l] in
+  let rp = repeati n f_sc ((state_spec_v st).[l], ()) in
 
   if n = 0 then begin
     eq_repeati0 n (update_block #a #m len b) st;
-    eq_repeati0 n f_sc (state_spec_v st).[l] end
+    eq_repeati0 n f_sc ((state_spec_v st).[l], ()) end
   else begin
     let lp1 = repeati (n - 1) (update_block #a #m len b) st in
-    let rp1 = repeati (n - 1) f_sc (state_spec_v st).[l] in
+    let rp1 = repeati (n - 1) f_sc ((state_spec_v st).[l], ()) in
     update_nblocks_loop_lemma #a #m len b st l (n - 1);
-    assert ((state_spec_v lp1).[l] == rp1);
+    assert ((state_spec_v lp1).[l] == Pervasives.fst rp1);
     unfold_repeati n (update_block #a #m len b) st (n - 1);
-    unfold_repeati n f_sc (state_spec_v st).[l] (n - 1);
+    unfold_repeati n f_sc ((state_spec_v st).[l], ()) (n - 1);
     update_block_lemma_l #a #m len b (n - 1) lp1 l end
 
 
@@ -641,7 +641,7 @@ val update_nblocks_lemma_l:
   -> l:nat{l < lanes a m} ->
   Lemma
    ((state_spec_v (update_nblocks len b st)).[l] ==
-    Spec.update_nblocks a len b.(|l|) (state_spec_v st).[l])
+    Pervasives.fst (Spec.update_nblocks a len b.(|l|) ((state_spec_v st).[l], ())))
 
 let update_nblocks_lemma_l #a #m len b st l =
   let blocks = len / block_length a in
